smartInfo starting to work

src/Symbolic/Expr/CmpInfo.v
@@ -1,7 +1,7 @@
 Require Import CoqStock.List.
 Require Export CoqStock.Cmp.
 
-Require Import Symbolic.Expr.Expr.
+Require Import Symbolic.Expr.Info.
 
 Fixpoint compare_info (x y: Info) {struct x} :=
   match x with
@@ -43,30 +43,37 @@ Theorem proof_info_compare_eq_implies_equal: forall (x y: Info)
   (c: compare_info x y = Eq)
   , x = y.
 Proof.
+intros.
+(*TODO*)
 Admitted.
 
 Theorem proof_info_compare_eq_reflex: forall (p: Info)
   , compare_info p p = Eq.
+(*TODO*)
 Admitted.
 
 Theorem proof_info_compare_eq_trans: forall (x y z: Info)
   (xy: compare_info x y = Eq)
   (yz: compare_info y z = Eq)
   , compare_info x z = Eq.
+(*TODO*)
 Admitted.
 
 Theorem proof_info_compare_lt_trans: forall (x y z: Info)
   (xy: compare_info x y = Lt)
   (yz: compare_info y z = Lt)
   , compare_info x z = Lt.
+(*TODO*)
 Admitted.
 
 Theorem proof_info_compare_gt_trans: forall (x y z: Info)
   (xy: compare_info x y = Gt)
   (yz: compare_info y z = Gt)
   , compare_info x z = Gt.
+(*TODO*)
 Admitted.
 
+#[export]
 Instance CmpInfo: Cmp (Info) :=
   {
     compare := compare_info
@@ -75,45 +82,4 @@ Instance CmpInfo: Cmp (Info) :=
   ; proof_compare_eq_trans := proof_info_compare_eq_trans
   ; proof_compare_lt_trans := proof_info_compare_lt_trans
   ; proof_compare_gt_trans := proof_info_compare_gt_trans
-  }.
-
-Definition compare_rexpr {A: Set} {B: Set} (x y: RExpr B): comparison :=
-  compare_info (@get_info A B x) (@get_info A B y).
-
-Theorem proof_rexpr_compare_eq_implies_equal: forall {A: Set} {B: Set} (x y: RExpr B)
-  (c: @compare_rexpr A B x y = Eq)
-  , x = y.
-Admitted.
-
-Theorem proof_rexpr_compare_eq_reflex: forall {A: Set} {B: Set} (p: RExpr B)
-  , @compare_rexpr A B p p = Eq.
-Admitted.
-
-Theorem proof_rexpr_compare_eq_trans: forall {A: Set} {B: Set} (x y z: RExpr B)
-  (xy: @compare_rexpr A B x y = Eq)
-  (yz: @compare_rexpr A B y z = Eq)
-  , @compare_rexpr A B x z = Eq.
-Admitted.
-
-Theorem proof_rexpr_compare_lt_trans: forall {A: Set} {B: Set} (x y z: RExpr B)
-  (xy: @compare_rexpr A B x y = Lt)
-  (yz: @compare_rexpr A B y z = Lt)
-  , @compare_rexpr A B x z = Lt.
-Admitted.
-
-Theorem proof_rexpr_compare_gt_trans: forall {A: Set} {B: Set} (x y z: RExpr B)
-  (xy: @compare_rexpr A B x y = Gt)
-  (yz: @compare_rexpr A B y z = Gt)
-  , @compare_rexpr A B x z = Gt.
-Admitted.
-
-#[export]
-Instance CmpRExpr {A: Set} {B: Set}: Cmp (RExpr B) :=
-  {
-    compare := @compare_rexpr A B
-  ; proof_compare_eq_implies_equal := proof_rexpr_compare_eq_implies_equal
-  ; proof_compare_eq_reflex := proof_rexpr_compare_eq_reflex
-  ; proof_compare_eq_trans := proof_rexpr_compare_eq_trans
-  ; proof_compare_lt_trans := proof_rexpr_compare_lt_trans
-  ; proof_compare_gt_trans := proof_rexpr_compare_gt_trans
   }.
