src/Symbolic/Expr/CmpRExpr.v
@@ -1,0 +1,51 @@
+Require Import CoqStock.List.
+Require Export CoqStock.Cmp.
+
+Require Import Symbolic.Expr.RExpr.
+
+
+Definition compare_rexpr {A: Set} {B: Set} (x y: RExpr B): comparison :=
+  compare_info (@get_info A B x) (@get_info A B y).
+
+Theorem proof_rexpr_compare_eq_implies_equal: forall {A: Set} {B: Set} (x y: RExpr B)
+  (c: @compare_rexpr A B x y = Eq)
+  , x = y.
+(*TODO*)
+Admitted.
+
+Theorem proof_rexpr_compare_eq_reflex: forall {A: Set} {B: Set} (p: RExpr B)
+  , @compare_rexpr A B p p = Eq.
+(*TODO*)
+Admitted.
+
+Theorem proof_rexpr_compare_eq_trans: forall {A: Set} {B: Set} (x y z: RExpr B)
+  (xy: @compare_rexpr A B x y = Eq)
+  (yz: @compare_rexpr A B y z = Eq)
+  , @compare_rexpr A B x z = Eq.
+(*TODO*)
+Admitted.
+
+Theorem proof_rexpr_compare_lt_trans: forall {A: Set} {B: Set} (x y z: RExpr B)
+  (xy: @compare_rexpr A B x y = Lt)
+  (yz: @compare_rexpr A B y z = Lt)
+  , @compare_rexpr A B x z = Lt.
+(*TODO*)
+Admitted.
+
+Theorem proof_rexpr_compare_gt_trans: forall {A: Set} {B: Set} (x y z: RExpr B)
+  (xy: @compare_rexpr A B x y = Gt)
+  (yz: @compare_rexpr A B y z = Gt)
+  , @compare_rexpr A B x z = Gt.
+(*TODO*)
+Admitted.
+
+#[export]
+Instance CmpRExpr {A: Set} {B: Set}: Cmp (RExpr B) :=
+  {
+    compare := @compare_rexpr A B
+  ; proof_compare_eq_implies_equal := proof_rexpr_compare_eq_implies_equal
+  ; proof_compare_eq_reflex := proof_rexpr_compare_eq_reflex
+  ; proof_compare_eq_trans := proof_rexpr_compare_eq_trans
+  ; proof_compare_lt_trans := proof_rexpr_compare_lt_trans
+  ; proof_compare_gt_trans := proof_rexpr_compare_gt_trans
+  }.
