src/Symbolic/Expr/CmpSmartInfo.v
@@ -1,0 +1,58 @@
+Require Import CoqStock.List.
+Require Export CoqStock.Cmp.
+
+Require Import Symbolic.Expr.CmpInfo.
+Require Import Symbolic.Expr.SmartInfo.
+
+Fixpoint compare_smart_info (x y: SmartInfo) {struct x} :=
+  match x with
+  | mkSmart x' _ =>
+    match y with
+    | mkSmart y' _ =>
+      CmpInfo.compare_info x' y'
+    end
+  end.
+
+Theorem proof_info_compare_eq_implies_equal: forall (x y: Info)
+  (c: compare_info x y = Eq)
+  , x = y.
+Proof.
+(*TODO*)
+Admitted.
+
+Theorem proof_info_compare_eq_reflex: forall (p: Info)
+  , compare_info p p = Eq.
+(*TODO*)
+Admitted.
+
+Theorem proof_info_compare_eq_trans: forall (x y z: Info)
+  (xy: compare_info x y = Eq)
+  (yz: compare_info y z = Eq)
+  , compare_info x z = Eq.
+(*TODO*)
+Admitted.
+
+Theorem proof_info_compare_lt_trans: forall (x y z: Info)
+  (xy: compare_info x y = Lt)
+  (yz: compare_info y z = Lt)
+  , compare_info x z = Lt.
+(*TODO*)
+Admitted.
+
+Theorem proof_info_compare_gt_trans: forall (x y z: Info)
+  (xy: compare_info x y = Gt)
+  (yz: compare_info y z = Gt)
+  , compare_info x z = Gt.
+(*TODO*)
+Admitted.
+
+#[export]
+Instance CmpInfo: Cmp (Info) :=
+  {
+    compare := compare_info
+  ; proof_compare_eq_implies_equal := proof_info_compare_eq_implies_equal
+  ; proof_compare_eq_reflex := proof_info_compare_eq_reflex
+  ; proof_compare_eq_trans := proof_info_compare_eq_trans
+  ; proof_compare_lt_trans := proof_info_compare_lt_trans
+  ; proof_compare_gt_trans := proof_info_compare_gt_trans
+  }.
