src/Symbolic/Expr/ExampleExpr.v
@@ -4,35 +4,30 @@ Require Import CoqStock.List.
 Require Import Symbolic.Expr.Expr.
 Require Import Symbolic.Expr.CmpExpr.
 
-
-
-(* TODO: Add a module implicit for A *)
+Require Import Symbolic.Input.BoolInput.
+Require Import Symbolic.Input.NatInput.
+Require Import Symbolic.Input.Result.
 
 Definition boolConst {A: Set} (v: bool): RExpr bool :=
-  smartRExpr (fun (_:A) => v) 0 [].
+  smartRExpr (fun (_:A) => ok v) 0 [].
 
-Definition boolVar: RExpr bool :=
-  smartRExprVar (fun (v:bool) => v) 1 [].
+Definition boolVar {A: Set} {b: BoolInput A}: RExpr bool :=
+  smartRExprVar getBool 1 [].
 
 Definition natConst {A: Set} (v: nat): RExpr nat :=
-  smartRExpr (fun (_:A) => v) 2 [].
+  smartRExpr (fun (_:A) => ok v) 2 [].
 
-Definition natVar: RExpr nat :=
-  (* TODO: how do we know A is nat, it could not be, see https://github.com/katydid/katydid/blob/master/parser/parser.go#L32 *)
-  smartRExprVar (fun (v:nat) => v) 3 [].
+Definition natVar {A: Set} {b: NatInput A}: RExpr nat :=
+  smartRExprVar getNat 3 [].
 
 Definition natEq {A: Set} (x y: RExpr nat): RExpr bool :=
-  let f := (fun (v: A)  => Nat.eqb (get_fn x v) (get_fn y v)) in
-  smartRExpr f 4 (map get_info [x; y]).
+  let f := (fun (v: A)  => swallow Nat.eqb (get_fn x v) (get_fn y v)) in
+  smartRExpr f 4 (map get_sinfo [x; y]).
 
-(* Definition andBool {A: Set} (x y: RExpr bool): RExpr bool :=
-  let f := (fun (v: A) => andb (get_fn x v) (get_fn y v)) in
-  smartRExpr f 5 (map get_info [x; y]). *)
-
-Definition smartAnd {A: Set} (x y: @RExpr nat bool): @RExpr bool bool :=
-  let f := (fun (v: A)  => andb (get_fn x v) (get_fn y v)) in
+Definition smartAnd {A: Set} (x y: RExpr bool): RExpr bool :=
+  let f := (fun (v: A)  => swallow andb (get_fn x v) (get_fn y v)) in
   match compare x y with
-  | Lt => smartRExpr f 5 (map get_info [x; y])
-  | Gt => smartRExpr f 5 (map get_info [y; x])
+  | Lt => smartRExpr f 5 (map get_sinfo [x; y])
+  | Gt => smartRExpr f 5 (map get_sinfo [y; x])
   | Eq => x
   end.
