src/Symbolic/Expr/Info.v
@@ -1,0 +1,86 @@
+Require Import CoqStock.Cmp.
+Require Import CoqStock.DubStep.
+Require Import CoqStock.List.
+Require Import CoqStock.Invs.
+
+(*
+  Info is the all the information about the Parsed expression.
+  This is mostly used to efficiently compare two expressions.
+  This includes a hash and whether the expression has a variable.
+*)
+Inductive Info: Type :=
+  mkInfo:
+    forall
+    (name: nat)
+    (params: list Info)
+    (hasvar: bool)
+    (hash: nat),
+  Info.
+
+(* Info: Getters *)
+
+Definition get_name (x: Info): nat :=
+  match x with
+  | mkInfo name _ _ _ => name
+  end.
+
+Definition get_params (x: Info): list Info :=
+  match x with
+  | mkInfo _ params _ _ => params
+  end.
+
+Definition get_hasvar (x: Info): bool :=
+  match x with
+  | mkInfo _ _ hasvar _ => hasvar
+  end.
+
+Definition get_hash (x: Info): nat :=
+  match x with
+  | mkInfo _ _ _ hash => hash
+  end.
+
+(* HasVar *)
+
+Fixpoint any (xs: list bool): bool :=
+  match xs with
+  | [] => false
+  | (x::xs) =>
+    match x with
+    | true => true
+    | _ => any xs
+    end
+  end.
+
+Definition has_var_from_params (params: list Info): bool :=
+  let param_hasvars := map get_hasvar params in
+  any param_hasvars.
+
+(* Hash *)
+
+Definition hash_per_elem (state: nat) (x: nat): nat :=
+    31 * state + x.
+
+Fixpoint hash_from_info (i: Info): nat :=
+  match i with
+  | mkInfo name params _ _ =>
+    let name_hashed := 31 * 17 * name in
+    let param_hashes := map hash_from_info params in
+    fold_left hash_per_elem param_hashes name_hashed
+  end.
+
+(* Defined for the purpose of a generalized proof *)
+
+(* hname is an already hashed name *)
+Definition hash_from_params (hname: nat) (params: list Info): nat :=
+  let param_hashes := map hash_from_info params in
+  fold_left hash_per_elem param_hashes hname.
+
+Definition hash_from_name_and_params (name: nat) (params: list Info): nat :=
+  hash_from_params (31 * 17 * name) params.
+
+Lemma same_hash_from_name_and_params_or_hash_from_info:
+  forall (name: nat) (params: list Info) (hasvar: bool) (hash: nat),
+  hash_from_name_and_params name params = hash_from_info (mkInfo name params hasvar hash).
+Proof.
+reflexivity.
+Qed.
