src/Symbolic/Expr/SmartInfo.v
@@ -1,0 +1,309 @@
+Require Import CoqStock.Cmp.
+Require Import CoqStock.DubStep.
+Require Import CoqStock.List.
+Require Import CoqStock.Invs.
+
+Require Import Symbolic.Expr.Info.
+
+(*
+  IsSmart indicates that Info was constructed with a smart constructor.
+*)
+
+Inductive IsSmartHash (i: Info): Prop :=
+  | isSmartHash :
+     get_hash i = hash_from_info i
+  -> Forall IsSmartHash (get_params i)
+  -> IsSmartHash i
+  .
+
+Inductive IsSmartHasVar (i: Info): Prop :=
+  | isSmartHasVar :
+     get_hasvar i = true
+  \/ get_hasvar i = has_var_from_params (get_params i)
+  -> Forall IsSmartHasVar (get_params i)
+  -> IsSmartHasVar i
+  .
+
+Inductive IsSmart (i: Info): Prop :=
+  | isSmart :
+     IsSmartHasVar i
+  -> IsSmartHash i
+  -> IsSmart i
+  .
+
+Inductive SmartInfo: Type :=
+  mkSmart:
+    forall
+    (info: Info)
+    (smart: IsSmart info),
+  SmartInfo.
+
+Definition get_info (s: SmartInfo): Info :=
+  match s with
+  | mkSmart info _ => info
+  end.
+
+(* Helper function for get_smart_params. *)
+Fixpoint get_smart_params' (params: list Info) (smartHasVars: Forall IsSmartHasVar params) (smartHashes: Forall IsSmartHash params): list SmartInfo.
+Proof.
+destruct params as [|p ps].
+- exact [].
+- apply Forall_cons_iff in smartHashes.
+  apply Forall_cons_iff in smartHasVars.
+  destruct smartHashes as [smartHash smartHashes].
+  destruct smartHasVars as [smartHasVar smartHasVars].
+  exact (
+    (mkSmart p (isSmart p smartHasVar smartHash))
+    :: (get_smart_params' ps  smartHasVars smartHashes)
+  ).
+Defined.
+
+(* Duplicate definition of get_smart_params' done using refine. *)
+Fixpoint get_smart_params''
+  (params: list Info)
+  (smartHasVars: Forall IsSmartHasVar params)
+  (smartHashes: Forall IsSmartHash params)
+  : list SmartInfo.
+Proof.
+refine (
+match params as params' return (Forall IsSmartHash params' -> Forall IsSmartHasVar params' -> list SmartInfo) with
+  | [] =>
+    fun (_ : Forall IsSmartHash []) (_ : Forall IsSmartHasVar []) => []
+  | (p::ps) =>
+      (fun
+        (smartHashes' : Forall IsSmartHash (p :: ps))
+        (smartHasVars' : Forall IsSmartHasVar (p :: ps)) =>
+          _
+      )
+end smartHashes smartHasVars
+).
+apply Forall_cons_iff in smartHashes'.
+apply Forall_cons_iff in smartHasVars'.
+destruct smartHashes' as [smartHash smartHashes'].
+destruct smartHasVars' as [smartHasVar smartHasVars'].
+exact (
+    (mkSmart p (isSmart p smartHasVar smartHash))
+    :: (get_smart_params' ps smartHasVars' smartHashes')
+  ).
+Defined.
+
+Theorem get_smart_params'_is_correct:
+  forall
+    (params: list Info)
+    (smartHasVars: Forall IsSmartHasVar params)
+    (smartHashes: Forall IsSmartHash params)
+  ,
+  map get_info (get_smart_params' params smartHasVars smartHashes)
+  =
+  params
+.
+Proof.
+intros.
+induction params as [| p ps].
+- reflexivity.
+- specialize (Forall_cons_iff IsSmartHash p ps) as Hiff.
+  inversion smartHashes.
+  subst.
+  rename H1 into smartHash.
+  rename H2 into smartHashes'.
+  inversion smartHasVars.
+  subst.
+  rename H1 into smartHasVar.
+  rename H2 into smartHasVars'.
+  specialize (IHps smartHasVars' smartHashes') as IHps.
+(* TODO *)
+Abort.
+
+Definition get_smart_params (s: SmartInfo): list SmartInfo.
+destruct s.
+destruct info.
+destruct smart as [smartHasVar smartHash].
+destruct smartHash as [_  smartHashes].
+destruct smartHasVar as [_ smartHasVars].
+cbn in *.
+exact (get_smart_params' params smartHasVars smartHashes).
+Defined.
+
+Theorem get_smart_params_is_correct:
+  forall (smart_info: SmartInfo),
+  map get_info (get_smart_params smart_info)
+  =
+  get_params (get_info smart_info)
+.
+Proof.
+intros.
+destruct smart_info.
+destruct info.
+dubstep get_params.
+destruct smart as [smartHasVar smartHash].
+destruct smartHash as [smartHash smartHashes].
+destruct smartHasVar as [smartHasVar smartHasVars].
+unfold get_smart_params.
+(* TODO *)
+Abort.
+
+(* hname is an already hashed name *)
+Definition hash_from_smart_params (hname: nat) (sparams: list SmartInfo) : nat :=
+  let param_hashes := map (fun sp => get_hash (get_info sp)) sparams in
+  fold_left hash_per_elem param_hashes hname.
+
+Lemma hash_from_params_is_hash_from_smart_params:
+  forall (hname: nat) (sparams: list SmartInfo),
+    hash_from_smart_params hname sparams
+    =
+    hash_from_params hname (map get_info sparams).
+Proof.
+intros.
+
+(* induction on params *)
+generalize dependent hname.
+induction sparams as [| sp sps].
+- reflexivity.
+- intros.
+
+(* step hash_from_params *)
+unfold hash_from_params.
+dubstep map.
+dubstep fold_left.
+assert (
+  fold_left
+    hash_per_elem
+    (map hash_from_info (map get_info sps))
+    (hash_per_elem hname (hash_from_info (get_info sp)))
+  =
+    hash_from_params (31 * hname + (get_hash (get_info sp))) (map get_info sps)
+) as Hinfo.
+destruct sp.
+destruct smart as [smartHasVar smartHash].
+destruct smartHash as [Heq Hforall].
+dubstep get_info.
+unfold hash_from_params.
+unfold hash_per_elem.
+rewrite Heq.
+reflexivity.
+rewrite Hinfo.
+clear Hinfo.
+
+(* step hash_from_smart_params *)
+unfold hash_from_smart_params.
+dubstep map.
+dubstep fold_left.
+assert (
+  fold_left
+    hash_per_elem
+    (map (fun sp' => get_hash (get_info sp')) sps)
+    (hash_per_elem hname (get_hash (get_info sp)))
+  =
+    hash_from_smart_params (31 * hname + (get_hash (get_info sp))) sps
+) as HsmartInfo.
+destruct sp.
+destruct smart as [smartHasVar smartHash].
+destruct smartHash as [Heq Hforall].
+dubstep get_info.
+unfold hash_from_smart_params.
+rewrite Heq.
+unfold hash_per_elem.
+reflexivity.
+rewrite HsmartInfo.
+clear HsmartInfo.
+
+apply IHsps.
+Qed.
+
+Definition has_var_from_smart_params (sparams: list SmartInfo): bool :=
+  let params := map get_info sparams in
+  let param_hasvars := map get_hasvar params in
+  any param_hasvars.
+
+(* get_smart_params (s: SmartInfo): list SmartInfo *)
+
+Definition forall_smart_has_var_from_smart_params
+  (sparams: list SmartInfo):
+  Forall IsSmartHasVar (map get_info sparams).
+induction sparams as [| p ps].
+- cbn. constructor.
+- cbn.
+  destruct p.
+  cbn.
+  constructor.
+  + destruct smart as [smartHasVar smartHash].
+    exact smartHasVar.
+  + exact IHps.
+Qed.
+
+Definition forall_smart_hash_from_smart_params
+  (sparams: list SmartInfo):
+  Forall IsSmartHash (map get_info sparams).
+induction sparams as [| p ps].
+- cbn. constructor.
+- cbn.
+  destruct p.
+  cbn.
+  constructor.
+  + destruct smart as [smartHasVar smartHash].
+    exact smartHash.
+  + exact IHps.
+Qed.
+
+Lemma is_smart_has_var (name: nat) (sparams: list SmartInfo) (has_var: bool):
+  IsSmartHasVar
+    (mkInfo
+      name
+      (map get_info sparams)
+      (has_var || has_var_from_smart_params sparams)
+      (hash_from_smart_params (31 * 17 * name) sparams)
+    ).
+Proof.
+apply isSmartHasVar.
+- destruct has_var.
+  + left.
+    cbn.
+    reflexivity.
+  + right.
+    cbn.
+    unfold has_var_from_smart_params.
+    reflexivity.
+- cbn.
+  apply forall_smart_has_var_from_smart_params.
+Qed.
+
+Lemma is_smart_hash (name: nat) (sparams: list SmartInfo) (has_var: bool):
+  IsSmartHash
+    (mkInfo
+      name
+      (map get_info sparams)
+      (has_var || has_var_from_smart_params sparams)
+      (hash_from_smart_params (31 * 17 * name) sparams)
+    ).
+Proof.
+apply isSmartHash.
+- dubstep get_hash.
+  dubstep hash_from_info.
+  rewrite hash_from_params_is_hash_from_smart_params.
+  unfold hash_from_params.
+  reflexivity.
+- cbn.
+  apply forall_smart_hash_from_smart_params.
+Qed.
+
+Definition smartInfo' (name: nat) (sparams: list SmartInfo) (has_var: bool): SmartInfo.
+exists
+  (mkInfo
+    name
+    (map get_info sparams)
+    (has_var || has_var_from_smart_params sparams)
+    (hash_from_smart_params
+      (31 * 17 * name)
+      sparams
+    )
+  ).
+apply isSmart.
+- apply is_smart_has_var.
+- apply is_smart_hash.
+Defined.
+
+Definition smartInfo (name: nat) (sparams: list SmartInfo): SmartInfo :=
+  smartInfo' name sparams false.
+
+Definition smartInfoVar (name: nat) (sparams: list SmartInfo): SmartInfo :=
+  smartInfo' name sparams true.
