src/Symbolic/Input/Input.v
@@ -1,11 +1,12 @@
 
 Require Import Symbolic.Input.BoolInput.
 Require Import Symbolic.Input.NatInput.
+Require Import Symbolic.Input.Result.
 
 Class Input (A: Type) :=
   {
-    getBool : A -> bool
-    ; getNat : A -> nat
+    getBool : A -> Result bool
+    ; getNat : A -> Result nat
   }.
 
 #[export]
@@ -27,32 +28,32 @@ Instance InputIsNatInput (A: Type) {i: Input A}: NatInput A :=
     getNat := getNat
   }.
 
-Definition boolConst {A: Set} (v: bool): A -> bool :=
-  fun _ => v.
+Definition boolConst {A: Set} (v: bool): A -> Result bool :=
+  fun _ => ok v.
 
-Definition boolVar {A: Set} {b: BoolInput A}: A -> bool :=
+Definition boolVar {A: Set} {b: BoolInput A}: A -> Result bool :=
   BoolInput.getBool.
 
-Definition natConst {A: Set} (v: nat): A -> nat :=
-  fun _ => v.
+Definition natConst {A: Set} (v: nat): A -> Result nat :=
+  fun _ => ok v.
 
-Definition natVar {A: Set} {n: NatInput A}: A -> nat :=
+Definition natVar {A: Set} {n: NatInput A}: A -> Result nat :=
   NatInput.getNat.
 
-Definition natEq {A: Set} (x y: A -> nat): A -> bool :=
-  fun (v: A)  => Nat.eqb (x v) (y v).
+Definition natEq {A: Set} (x y: A -> Result nat): A -> Result bool :=
+  fun (v: A) => swallow Nat.eqb (x v) (y v).
 
-Definition andBool {A: Set} (x y: A -> bool): A -> bool :=
-  fun (v: A) => andb (x v) (y v).
+Definition andBool {A: Set} (x y: A -> Result bool): A -> Result bool :=
+  fun (v: A) => swallow andb (x v) (y v).
 
-Definition example_expr1 {A: Set}: A -> bool :=
+Definition example_expr1 {A: Set}: A -> Result bool :=
   andBool (boolConst true) (boolConst false).
 
-Definition example_expr2 {A: Set} {b: BoolInput A}: A -> bool :=
+Definition example_expr2 {A: Set} {b: BoolInput A}: A -> Result bool :=
   andBool boolVar (boolConst false).
 
-Definition example_expr3 {A: Set} {i: Input A}: A -> bool :=
+Definition example_expr3 {A: Set} {i: Input A}: A -> Result bool :=
   andBool boolVar (boolConst false).
 
-Definition example_expr4 {A: Set} {i: Input A}: A -> bool :=
+Definition example_expr4 {A: Set} {i: Input A}: A -> Result bool :=
   andBool (natEq natVar (natConst 1)) boolVar.
