src/Symbolic/Input/NatInput.v
@@ -1,12 +1,14 @@
+Require Import Symbolic.Input.Result.
+
 Class NatInput (A: Type) :=
   {
-    getNat : A -> nat
+    getNat : A -> Result nat
   }.
 
 #[export]
 Instance NatIsNatInput: NatInput nat :=
   {
-    getNat := fun (n: nat) => n
+    getNat := fun (n: nat) => ok n
   }.
 
 #[export]
@@ -14,7 +16,7 @@ Instance BoolIsNatInput: NatInput bool :=
   {
     getNat := fun (b: bool) =>
       match b with
-      | false => 0
-      | true => 1
+      | false => ok 0
+      | true => ok 1
       end
   }.
